fiat2/src/fiat2/DictIndexImplEx2.v
@@ -1,0 +1,124 @@
+Require Import fiat2.Language fiat2.Interpret fiat2.Value fiat2.TypeSystem fiat2.TypeSound fiat2.IndexInterface
+fiat2.CollectionTransf fiat2.DictIndexImpl2 fiat2.TransfUtils fiat2.RelTransf fiat2.IndexTransf2 fiat2.TransfSound fiat2.Utils fiat2.Substitute.
+Require Import coqutil.Map.Interface coqutil.Map.SortedListString coqutil.Word.Interface coqutil.Datatypes.Result.
+Require Import List String ZArith.
+Import ListNotations.
+
+Section ConcreteExample.
+  Context {width: Z} {word: word.word width} {word_ok: word.ok word}.
+  Notation value := (value (width:=width)).
+
+  Local Open Scope string.
+
+  Instance ctenv : map.map string type := SortedListString.map _.
+  Instance ctenv_ok : map.ok ctenv := SortedListString.ok _.
+
+  Instance clocals : map.map string value := SortedListString.map _.
+  Instance clocals_ok : map.ok clocals := SortedListString.ok _.
+
+  Instance caenv : map.map string collection_tag := SortedListString.map _.
+  Instance caenv_ok : map.ok caenv := SortedListString.ok _.
+
+  Instance cRenv : map.map string (value -> value -> Prop) := SortedListString.map _.
+  Instance cRenv_ok : map.ok cRenv := SortedListString.ok _.
+
+  Definition attr := "department".
+
+  Notation idx_wf := (idx_wf "hole" attr "tup" "acc" "x").
+  Instance cdict_idx : IndexInterface2.index := (dict_idx "hole" attr "tup" "acc" "x").
+  Instance cdict_idx_ok : IndexInterface2.ok cdict_idx idx_wf.
+  apply dict_idx_ok. auto with transf_hints.
+  Qed.
+
+  Definition to_filter_transf := fold_command id to_filter_head.
+  Definition annotate_collection_transf := fold_command id annotate_collection.
+  Definition push_down_collection_transf := fold_command id push_down_collection.
+  Definition lookup_transf := fun tbl => fold_command_with_globals [tbl] (eq_filter_to_lookup_head attr "id_tag" "aux_tag" "dict_idx_tag" "b" tbl).
+  Definition cons_transf := fun tbl => fold_command_with_globals [tbl] (cons_to_insert_head attr "tup" "acc" "x" "y").
+  Definition use_dict_idx_transf := fun tbl => fold_command_with_globals [tbl] (use_idx_head attr "id_tag" "aux_tag" "dict_idx_tag" tbl).
+
+  Notation idxs := [("dict_idx_tag", cdict_idx, idx_wf)].
+  Instance ccompo_idx : IndexInterface2.index := compo_idx idxs "hole" (word:=word).
+  Instance ccompo_idx_ok : IndexInterface2.ok ccompo_idx (compo_idx_wf idxs).
+  apply compo_idx_ok; repeat constructor; auto; intros.
+  1: apply idx_ty_wf; auto.
+  1: apply to_idx_ty; auto with transf_hints.
+  Qed.
+
+  Definition ex_transf (Gstore Genv : ctenv) :=
+    Basics.compose (apply_idx_related_transfs (idx:=ccompo_idx) "id_tag" "aux_tag" (fun tbl => Basics.compose (use_dict_idx_transf tbl) (Basics.compose (cons_transf tbl) (Basics.compose (cons_transf tbl) (lookup_transf tbl)))) Gstore Genv) (Basics.compose push_down_collection_transf (Basics.compose annotate_collection_transf to_filter_transf)).
+
+  Hint Extern 5 ((_ : string) <> _) => apply eqb_neq; auto : transf_hints.
+  Hint Resolve push_down_collection_sound : transf_hints.
+  Hint Resolve annotate_collection_sound : transf_hints.
+  Hint Resolve use_idx_head_sound : transf_hints.
+  Hint Extern 5 (forall v, aux_wf _ _ v -> DictIndexImpl2.aux_wf_for_idx _ _ _ _ _ _ _ _ v) =>
+              intros; unfold aux_wf, aux_wf_for_idx, compo_idx_wf in *;
+              repeat destruct_match_hyp; intuition idtac;
+              invert_Forall; unfold idx_wf, record_proj in *;
+                             destruct_match_hyp; intuition eauto : transf_hints.
+  Hint Extern 5 (aux_ty_for_idx _ _ _ _ _) => unfold aux_ty_for_idx, aux_ty; cbn; auto : transf_hints.
+  Hint Extern 5 (forall t, IndexInterface2.is_tbl_ty t = true -> _ = true) =>
+         unfold IndexInterface2.is_tbl_ty; cbn; intros;
+  rewrite Bool.andb_true_iff in *; intuition auto : transf_hints.
+  Hint Extern 5 string => pose proof ("":string). (* ??? : transf_hints doesn't work; how to find the cause of this extra arg? *)
+  Hint Resolve cons_to_insert_head_sound : transf_hints.
+  Hint Extern 5 (expr_aug_transf_sound _ _ _ (DictIndexImpl2.use_idx_head _ _ _ _)) =>
+         eapply use_idx_head_sound; [ | | | | | | eauto with transf_hints ]; auto with transf_hints : transf_hints.
+  Hint Extern 5 (expr_aug_transf_sound _ _ _ (DictIndexImpl2.eq_filter_to_lookup_head _ _ _ _ _)) =>
+         eapply eq_filter_to_lookup_head_sound; [ | | | | | | eauto with transf_hints ]; auto with transf_hints : transf_hints.
+  Hint Extern 5 (transf_sound (apply_idx_related_transfs _ _ _)) => apply apply_idx_related_transfs_sound : transf_hints.
+  Hint Extern 5 (@transf_sound width word ctenv clocals ex_transf) => apply transf_sound_compose : transf_hints. (* ??? Doesn't work *)
+
+  Lemma ex_transf_sound : transf_sound (locals:=clocals) ex_transf.
+  Proof.
+    apply transf_sound_compose; eauto 20 with transf_hints.
+  Qed.
+
+  Require Import fiat2.Notations.
+  Open Scope fiat2_scope.
+
+  Definition row_ty := TRecord (record_sort [("name", TString); ("department", TString); ("feedback", TString)]).
+  (* two arbitrary well_typed rows *)
+  Definition row1 := EVar "row1".
+  Definition row2 := EVar "row2".
+
+  Definition build_responses1 := <{ set "responses" := row1 :: row2 :: mut "responses" }>.
+  Definition filter_responses dpt : expr := ESort LikeList <[ "row" <- mut "responses" ;
+                                                       check("row"["department"] == << EAtom (AString dpt) >>);
+                                                       ret "row" ]>.
+  Definition query := CForeach (filter_responses "EECS") "r"
+                      <{ let "name" = "r"["name"] +++ << EAtom (AString ": ") >> in
+                         let "feedback" = "r"["feedback"] +++ << EAtom (AString "\n") >> in
+                         let "line" = "name" +++ "feedback" in
+                         set "all_feedback" := mut "all_feedback" +++ "line" }>.
+  Definition ex1' := CSeq build_responses1 query.
+  Definition ex1 := CLetMut (EAtom (ANil (Some (row_ty)))) "responses" ex1'.
+
+  Definition init_Gstore : ctenv := map.put map.empty "all_feedback" TString.
+  Definition init_Genv : ctenv := map.put (map.put map.empty "row1" row_ty) "row2" row_ty.
+
+  Definition ex1_1 := (Basics.compose push_down_collection_transf (Basics.compose annotate_collection_transf to_filter_transf)) ex1.
+  Compute ex1_1.
+  Compute apply_idx_related_transfs (idx:=ccompo_idx) "id_tag" "aux_tag" (fun tbl => Basics.compose (cons_transf tbl) (lookup_transf tbl)) init_Gstore init_Genv ex1_1.
+
+  Unset Printing Notations.
+  Definition ex1_transformed := ex_transf init_Gstore init_Genv ex1.
+  Compute ex1_transformed.
+
+  Ltac resolve_NoDup := repeat constructor; simpl; intuition idtac; congruence.
+
+  Ltac resolve_tenv_wf := repeat apply tenv_wf_step; try apply tenv_wf_empty; repeat constructor; resolve_NoDup.
+
+  Hint Extern 5 (well_typed _ _ _) => simple eapply command_typechecker_sound.
+  Hint Extern 5 (tenv_wf _) => resolve_tenv_wf.
+  Hint Extern 5 (typecheck _ _ _ = Success _) => reflexivity.
+
+  Theorem ex1_transformed_sem : forall (store env : clocals),
+      locals_wf init_Gstore store ->
+      locals_wf init_Genv env ->
+      interp_command store env ex1_transformed = interp_command store env ex1.
+  Proof.
+    eauto using transf_sound__preserve_sem, ex_transf_sound.
+  Qed.
+End ConcreteExample.
